Sorting/MergeSortSpec.v
@@ -1,14 +1,13 @@
 Require Import MergeSort.
-(*Require Import InsertionSort.*)
 
 Set Implicit Arguments.
 
 Theorem Sorted_ghms :
   forall (n : nat) (A : LinDec)
     (s : Sort A) (split : Split A)
-      (l : list A), Sorted A (@ghms n A (@sort A s) split l).
+      (l : list A), Sorted A (@ghms n A (@sort A A s) split l).
 Proof.
-  intros. functional induction @ghms n A (@sort A s) split l.
+  intros. functional induction @ghms n A (@sort A A s) split l.
     destruct s; cbn in *. apply Sorted_sort.
     apply Sorted_merge; cbn; assumption.
 Qed.
@@ -16,9 +15,9 @@ Qed.
 Theorem ghms_perm :
   forall (n : nat) (A : LinDec)
     (s : Sort A) (split : Split A)
-      (l : list A), perm A l (@ghms n A (@sort A s) split l).
+      (l : list A), perm l (@ghms n A (@sort A A s) split l).
 Proof.
-  intros. functional induction @ghms n A (@sort A s) split l.
+  intros. functional induction @ghms n A (@sort A A s) split l.
     apply sort_perm.
     rewrite perm_split_app. rewrite e0; cbn.
       rewrite <- merge_perm; cbn. apply perm_app; assumption.
@@ -26,9 +25,9 @@ Qed.
 
 Theorem Permutation_ghms :
   forall (n : nat) (A : LinDec) (s : Sort A) (split : Split A) (l : list A),
-    Permutation (@ghms n A (@sort A s) split l) l.
+    Permutation (@ghms n A (@sort A A s) split l) l.
 Proof.
-  intros. functional induction @ghms n A (@sort A s) split l.
+  intros. functional induction @ghms n A (@sort A A s) split l.
     apply Permutation_sort.
     rewrite <- (@Permutation_app_split _ _ l). rewrite e0; cbn.
       rewrite <- Permutation_merge. cbn. apply Permutation_app; assumption.
